Compiler: WIP - Poseidon

Clap/Compiler/Traverse.lean
@@ -1,6 +1,11 @@
 import Lean
 import Qq
 
+import Lean.Meta.Sym.SymM
+import Lean.Meta.Tactic.Cbv.Main
+
+import Clap.Lang
+import Clap.Spec
 import Clap.Compiler.Simp
 import Clap.Compiler.Vectors
 import Clap.Compiler.Wheels
@@ -11,17 +16,97 @@ open Lean Meta Qq Elab
 
 abbrev ExprS := Expr × Expr ⊕ Expr
 
-def ExprS.pretty (e : ExprS) : MetaM String := do
+def matchBinds (e : Expr) : Option (Expr × Expr) :=
+  if let (``Bind.bind, ⟨_ :: _ :: _ :: _ :: e :: k :: _⟩) := e.getAppFnArgs then some (e, k)
+  else
+  if let (``Option.bind, ⟨_ :: _ :: e :: k :: []⟩) := e.getAppFnArgs then some (e, k)
+  else none
+
+/--
+For the purposes of reporting, we bias chains of non-ground expressions to the right.
+-/
+partial def isGroundTerm (e : Expr) : Sym.Simp.SimpM (Option Expr) := do
+  if let .lam name type body bi := e then
+    withLocalDecl name bi type fun fvar =>
+      isGroundTerm (body.instantiate1 fvar)
+  else
+  if let some (e,k) := matchBinds e then
+    return andThen (←isGroundTerm e) (←isGroundTerm k)
+  else
+  if let (``Option.some, ⟨_ :: e :: _⟩) := e.getAppFnArgs then
+    isGroundTerm e
+  else
+  if let (``Pure.pure, ⟨_ :: _ :: _ :: e :: _⟩) := e.getAppFnArgs then
+    isGroundTerm e
+  else
+  if let (``Clap.Lang.Core.eq0, ⟨_ :: _ :: e :: _⟩) := e.getAppFnArgs then
+    isGroundTerm e
+  else
+  if let (``Clap.Lang.Core.num2bits, ⟨_ :: _ :: _ :: e :: _⟩) := e.getAppFnArgs then
+    isGroundTerm e
+  else
+  if let (``Clap.Lang.Core.isZero, ⟨_ :: _ :: e :: _⟩) := e.getAppFnArgs then
+    isGroundTerm e
+  else
+  if let (``Clap.Lang.Core.share, ⟨_ :: _ :: e :: _⟩) := e.getAppFnArgs then
+    isGroundTerm e
+  else
+  if let (``Vector.mk, ⟨_ :: _ :: e :: _ :: _⟩) := e.getAppFnArgs then
+    isGroundTerm e
+  else
+  if let (``Array.mk, ⟨_ :: e :: _⟩) := e.getAppFnArgs then
+    isGroundTerm e
+  else
+  if let (``List.toArray, ⟨_ :: e :: _⟩) := e.getAppFnArgs then
+    isGroundTerm e
+  else
+  if let (``List.nil, _) := e.getAppFnArgs then
+    return .none
+  else
+  if let (``List.cons, ⟨_ :: hd :: tl :: _⟩) := e.getAppFnArgs then
+    return andThen (←isGroundTerm hd) (←isGroundTerm tl)
+  if let (``OfNat.ofNat, _) := e.getAppFnArgs then
+    return .none
+  else
+  if let .fvar _ := e then
+    return .none
+  else
+  if let (``GetElem.getElem, ⟨_ :: _ :: _ :: _ :: _ :: coll :: elem :: _ :: _⟩) := e.getAppFnArgs then -- TODO: Do we want to allow only `<circuit input>[i]`?
+    return andThen (if coll.isFVar then .none else .some e) (←isGroundTerm elem)
+  else
+  if let (``HAdd.hAdd, ⟨_ :: _ :: _ :: _ :: l :: r :: _⟩) := e.getAppFnArgs then
+    let l ← isGroundTerm l
+    let r ← isGroundTerm r
+    return andThen l r
+  else
+  if let (``HMul.hMul, ⟨_ :: _ :: _ :: _ :: l :: r :: _⟩) := e.getAppFnArgs then
+    let l ← isGroundTerm l
+    let r ← isGroundTerm r
+    return andThen l r
+  else
+  if let (``HSub.hSub, ⟨_ :: _ :: _ :: _ :: l :: r :: _⟩) := e.getAppFnArgs then
+    let l ← isGroundTerm l
+    let r ← isGroundTerm r
+    return andThen l r
+  else
+    return .some e
+  where andThen (e₁ e₂ : Option Expr) : Option Expr :=
+    match e₁, e₂ with
+    | .none, .none => .none
+    | .none, .some e | .some e, .none => .some e
+    | .some _, .some e => .some e
+
+def ExprS.pretty (e : ExprS) : Sym.Simp.SimpM String := do
   match e with
   | .inl (e, binder) => return s!"λ {binder} ↦ {←PrettyPrinter.ppExpr e}"
   | .inr e => PrettyPrinter.ppExpr e <&> Format.pretty
 
-def _root_.Lean.Expr.isBind (e : Expr) : MetaM Bool := do
+def _root_.Lean.Expr.isBind (e : Expr) : Sym.Simp.SimpM Bool := do
   return e.isAppOf ``Bind.bind || e.isAppOf ``Option.bind
 
-def _root_.Lean.Expr.getBindArgs? (e : Expr) : MetaM (Option (Expr × Expr)) := do
+def _root_.Lean.Expr.getBindArgs? (e : Expr) : Sym.Simp.SimpM (Option (Expr × Expr)) := do
   -- If `e` is not `λ _ ↦ _`, then `lambdaTelescope = id`.
-  lambdaTelescope e fun _ e ↦ do
+  lambdaTelescope e fun arg e ↦ do
     if !(←e.isBind) then return .none
     let firstExplicitArg := (←getFunInfo e.getAppFn).paramInfo.findIdx (·.binderInfo.isExplicit)
     let bindArgs := e.getAppArgs
@@ -30,16 +115,29 @@ def _root_.Lean.Expr.getBindArgs? (e : Expr) : MetaM (Option (Expr × Expr)) := 
       bindArgs[firstExplicitArg + 1]!
     )
 
-def _root_.Lean.Expr.mkBind (l r : Expr) (m? : Name := ``Bind.bind) : MetaM Expr := do
+def _root_.Lean.Expr.mkBind (l r : Expr) (m? : Name := ``Option.bind) : Sym.Simp.SimpM Expr := do
   mkAppM m? #[l, r]
 
 private def treeEmoji : String := "🌲"
+private def stopEmoji : String := "🛑"
+
+instance {m} [Monad m] : Union (m Sym.Simp.Methods) where
+  union a b := do return (←a) ∪ (←b)
+
+def isUnital (e : Expr) : Sym.Simp.SimpM Bool := do
+  let eT ← inferType e
+  if ← isDefEq eT q(Unit) then return true
+  let_expr Vector _ sz := eT | return false
+  let sz' ← Sym.simp sz
+  match (sz'.getResultExpr sz).nat? with
+  | .none => throwError m!"{sz} does not simplify to ground.\nExpr:\n{e}"
+  | .some n => return n == 0
 
 mutual
 
-private partial def down (reduce : Expr → TermElabM Expr)
-                         (reduceOuter : Expr → TermElabM Expr)
-                         (stack : List ExprS) (todo : Expr) : TermElabM Expr := do
+private partial def down (reduce : Expr → Sym.Simp.SimpM Expr)
+                         (reduceOuter : Expr → Sym.Simp.SimpM Expr)
+                         (stack : List ExprS) (todo : Expr) : Sym.Simp.SimpM Expr := do
   if let .some (l, r) ← todo.getBindArgs?
   then
     trace[Clap.Compile.down] "\npush [→]:\n{r}\ngo [↓]:\n{l}"
@@ -52,16 +150,21 @@ private partial def down (reduce : Expr → TermElabM Expr)
       trace[Clap.Compile.down] "\ngo [↓]:\n{simped}"
       down reduce reduceOuter stack simped
     else
-      trace[Clap.Compile.simp] "[↓] {crossEmoji}\n{todo}"
+      trace[Clap.Compile.simp.fail] "[↓] {crossEmoji}\n{todo}"
       trace[Clap.Compile.down] "\ngo [↑]:\n{todo}"
+      match ←isGroundTerm todo with
+      | .some e => trace[Clap.Compile.simp.warnDownNotGround] "{stopEmoji} [↓] stopped:\n{e}"
+      | .none => pure ()
       up reduce reduceOuter stack todo
 
-private partial def up (reduce : Expr → TermElabM Expr)
-                       (reduceOuter : Expr → TermElabM Expr)
-                       (stack : List ExprS) (done : Expr) : TermElabM Expr := do
+private partial def up (reduce : Expr → Sym.Simp.SimpM Expr)
+                       (reduceOuter : Expr → Sym.Simp.SimpM Expr)
+                       (stack : List ExprS) (done : Expr) : Sym.Simp.SimpM Expr := do
   match stack with
   | [] =>
     trace[Clap.Compile.up] "Done"
+    trace[Clap.Compile.up]
+      "This should go to debug tracing. Simped done:\n{←reduce done}"
     return done
   | .inr r :: stack =>
     lambdaTelescopeOne! r fun arg body ↦ do
@@ -70,47 +173,110 @@ private partial def up (reduce : Expr → TermElabM Expr)
   | .inl l :: stack => do
     let bind ← mkBindWith l done
     let up := up reduce reduceOuter stack
-    if ← isDefEq (←inferType l.2) q(Unit)
+    if ← isUnital l.2
     then trace[Clap.Compile.up] "\ngo [↑]:\n{bind}"
          up bind
-    else trace[Clap.Compile.simp] "Binding value: {l.2}"
-
+    else trace[Clap.Compile.simp] "Binding value: {l.2} {bind}"
          let simped ← reduceOuter bind
+        --  trace[Clap.Compile.simp] "WE MADE IT"
          if simped != bind
          then trace[Clap.Compile.simp] "[↑] {checkEmoji}\n{bind}\n==>\n{simped}"
-         else trace[Clap.Compile.simp] "[↑] {crossEmoji}\n{bind}"
-
+         else trace[Clap.Compile.simp.fail] "[↑] {crossEmoji}\n{bind}"
          trace[Clap.Compile.up] "\ngo [↑]:\n{simped}"
          up simped
   where mkBindWith (stackEntry : Expr × Expr) (cont : Expr)
-                   (m? : Name := ``Bind.bind) : MetaM Expr := do
-    mkLambdaFVars #[stackEntry.2] cont >>= stackEntry.1.mkBind (m? := m?)
+                   (m? : Name := ``Option.bind) : Sym.Simp.SimpM Expr := do
+    Sym.mkLambdaFVarsS #[stackEntry.2] cont >>= stackEntry.1.mkBind (m? := m?)
 
 end
 
-open Simp API
-
-def compile (e : Expr) (simpset : SimpSet) (only : Bool := true) : TermElabM Expr := do
+open Simp API in
+def compile (e : Expr) (simpset : Sym.Simp.Methods) : Sym.Simp.SimpM Expr := do
   withTraceNode `Clap.Compile formatExprWith do
-  trace[Clap.Compile.simp.config]
-    m!"Reducer: [only := {only}, singlePass := {true}, set := {repr simpset}"
-  trace[Clap.Compile.simp.config]
-    m!"Compiler: [only := true, singlePass := {false}, set := {repr compilerSet} ∪ {repr simpset}"
-  
   lambdaTelescope e fun args e ↦ do
-    let compiled ←
-      down (simplify (only := only) (singlePass := true) simpset)
-           (simplify (only := true) (compilerSet.union simpset)) [] e
-    mkLambdaFVars args compiled
+    let compiled ← down
+      (reduce      := simplify simpset)
+      (reduceOuter := simplify (simpset ∪ (←compilerSet)))
+      (stack       := [])
+      (todo        := e)
+    Sym.mkLambdaFVarsS args compiled
   where
-    compilerSet : SimpSet :=
-      SimpSet.withAllPost #[
+    compilerSet : MetaM Sym.Simp.Methods :=
+      Sym.mkMethods #[
         ``Option.bind_assoc, ``bind_assoc,
         ``Option.pure_def,
-        ``Option.bind_eq_bind, ``Option.bind_fun_some, ``Option.bind_some, ``bind_pure, ``pure_bind
+        ``Option.bind_eq_bind, ``Option.bind_fun_some, ``Option.bind_some, ``bind_pure, ``pure_bind,
+        ``Option.map_eq_map, ``Option.map_some
       ]
 
 namespace CompileSets
+
+section
+
+open Simp API
+
+namespace Logic
+
+def cases :=
+  SimpSet.withAllPost #[
+    ``dite_false, ``ite_false,
+
+    ``dite_true, ``ite_true    
+  ]
+
+end Logic
+
+namespace Nat
+
+def arith :=
+  SimpSet.withAllPost #[
+    ``Nat.reduceMul, ``Nat.reduceDiv,
+    ``Nat.reduceAdd, ``Nat.reduceSub,
+    ``Nat.zero_add, ``Nat.add_zero,
+    ``Nat.one_mul, ``Nat.mul_one
+  ]
+
+end Nat
+
+namespace List
+
+dsimproc_decl reduceRange (List.range _) := fun e ↦ do
+  let_expr _root_.List.range k ← e | return .continue
+  let ctx ← Simp.getContext
+  let ctx ← ctx.setConfig {ctx.config with singlePass := false}
+  withTheReader Simp.Context (fun _ ↦ ctx) do
+  match (←simp k).expr.nat? with
+  | .none => logError m!"{(←simp k).expr} is not ground"
+             return .done e
+  | .some n => let l := _root_.List.range n
+               return .visit (Lean.toExpr l)
+
+def range : SimpSet :=
+  {
+    pos := #[(``reduceRange, .Pre)]
+  }
+
+end List
+
+namespace Array
+
+dsimproc_decl reduceRange (Array.range _) := fun e ↦ do
+  let_expr _root_.Array.range k ← e | return .continue
+  let ctx ← Simp.getContext
+  let ctx ← ctx.setConfig {ctx.config with singlePass := false}
+  withTheReader Simp.Context (fun _ ↦ ctx) do
+  match (←simp k).expr.nat? with
+  | .none => logError m!"{(←simp k).expr} is not ground"
+             return .done e
+  | .some n => let l := _root_.Array.range n
+               return .visit (Lean.toExpr l)
+
+def range : SimpSet :=
+  {
+    pos := #[(``reduceRange, .Pre)]
+  }
+
+end Array
 
 namespace Vector
 
@@ -133,12 +299,22 @@ def getElem : SimpSet :=
     ``List.getElem_cons_zero, ``List.getElem_cons_succ,
   ]
 
+-- example {inputs : Vector Nat 2} {a} {a_2} : #v[a, #v[a_2 * (inputs[1] + 66)][0]] = sorry := by
+  -- rw [Vector.getElem_mk]
+
+  -- simp +singlePass only [Vector.getElem_mk, List.getElem_toArray, List.getElem_cons_zero]
+
+def mapOptim : SimpSet :=
+  {
+    pos := #[(``List.map_id, .Pre)]
+  }    
+
 def map : SimpSet :=
   SimpSet.withAllPost #[
     ``Vector.map_mk, ``List.map_toArray,
     
     ``List.map_cons, ``List.map_nil
-  ]
+  ] ∪ mapOptim
 
 def mapIdx : SimpSet :=
   SimpSet.withAllPost #[
@@ -154,19 +330,41 @@ def zipWith : SimpSet :=
     ``List.zipWith_cons_cons, ``List.zipWith_nil_left, ``List.zipWith_nil_right
   ]
 
+-- dsimproc_decl rwMk_append_mk (Vector.mk _ _ ++ Vector.mk _ _) := fun e ↦ do
+--   let x ← e.runTactic (←`(tactic| rw [$(mkIdent ``Vector.mk_append_mk):ident]))
+--   return .visit x
+
+-- def append : SimpSet :=
+--   SimpSet.withAllPost #[
+--     ``rwMk_append_mk, ``List.append_toArray, -- ``Vector.mk_append_mk
+
+--     ``List.cons_append, ``List.nil_append
+--   ]
+
+dsimproc_decl rwMk_append_mk (Vector.mk _ _ ++ Vector.mk _ _) := fun e ↦ do
+  let x ← e.runTactic (←`(tactic| rw [$(mkIdent ``Vector.mk_append_mk):ident]))
+  return .visit x
+
 def append : SimpSet :=
   SimpSet.withAllPost #[
     ``Vector.mk_append_mk, ``List.append_toArray,
 
-    ``List.cons_append, ``List.nil_append
+    ``List.cons_append, ``List.nil_append,
+
+    ``List.append_nil
   ]
 
 def take : SimpSet :=
   SimpSet.withAllPost #[
     ``Vector.take_mk, ``List.take_toArray,
 
-    ``List.take_succ_cons, ``List.take_nil
-    -- ``List.take_cons, ``List.take_nil
+    ``List.take_succ_cons, ``List.take_nil, ``List.take_zero
+  ]
+
+def size : SimpSet :=
+  SimpSet.withAllPost #[
+   ``Vector.size_toArray, ``List.size_toArray,
+   ``List.length_cons, ``List.length_nil
   ]
 
 theorem _root_.List.drop_toArray {α} {l : List α} {i} :
@@ -181,8 +379,21 @@ def drop : SimpSet :=
   SimpSet.withAllPost #[
     ``Vector.drop_mk, ``_root_.List.drop_toArray,
 
-    -- ``List.drop_cons, ``List.drop_nil,
-    ``List.drop_succ_cons, ``List.drop_zero, ``List.drop_nil
+    ``List.drop_succ_cons, ``List.drop_zero, ``List.drop_nil, ``List.drop_zero
+  ]
+
+def extract : SimpSet :=
+  SimpSet.withAllPost #[
+    ``Vector.extract_mk, ``List.extract_toArray,
+    
+    ``List.extract_eq_take_drop
+  ] ∪ drop ∪ take 
+
+def set : SimpSet :=
+  SimpSet.withAllPost #[
+    ``Vector.set_mk, ``List.set_toArray,
+    
+    ``List.set_cons_succ, ``List.set_cons_zero,
   ]
 
 def foldl : SimpSet :=
@@ -192,12 +403,18 @@ def foldl : SimpSet :=
     ``List.foldl_cons, ``List.foldl_nil
   ]
 
+dsimproc_decl erwFoldr_toArray (Array.foldr _ _ _ _ _) := fun e ↦ do
+  let_expr Array.foldr _ _ _ _ arr _ _ := e | return .continue
+  let_expr List.toArray _ _ := arr | return .continue
+  let x ← e.runTactic (←`(tactic| erw [$(mkIdent ``List.foldr_toArray):ident]))
+  return .visit x
+
 def foldr : SimpSet :=
   SimpSet.withAllPost #[
-    ``Vector.foldr_mk, ``List.foldr_toArray,
+    ``Vector.foldr_mk, ``erwFoldr_toArray,
 
     ``List.foldr_cons, ``List.foldr_nil
-  ]
+  ] ∪ size
 
 def sum : SimpSet :=
   SimpSet.withAllPost #[
@@ -205,48 +422,701 @@ def sum : SimpSet :=
   ] ∪ foldr
 
 @[simp]
-theorem _root_.Vector.mapM_singleton {α β} {m} [Monad m] [LawfulMonad m] {f : α → m β} {x} :
-  #v[x].mapM f = (#v[·]) <$> f x := by
+theorem _root_.Vector.mapM_singleton {α} {β} {m} [Monad m] [LawfulMonad m] {f : α → m β} {x} :
+  #v[x].mapM f = f x >>= (pure #v[·]) := by
   apply Vector.map_toArray_inj.mp; simp
 
+@[simp]
+theorem _root_.Vector.mapM_nil {α β} {m} [Monad m] [LawfulMonad m] {f : α → m β} :
+  #v[].mapM f = pure #v[] := by simp
+
 @[simp↓ high]
-theorem _root_.Vector.mapM_mk_singleton_append {m} [Monad m] [LawfulMonad m] {α β} {n} {f : α → m β}
-  (v : Vector α n) {x : α} :
+theorem _root_.Vector.mapM_mk_singleton_append {m} [Monad m] [LawfulMonad m] {α} {β} {n} {f : α → m β}
+  {v : Vector α n} {x : α} :
   (#v[x] ++ v).mapM f = (return #v[(←f x)] ++ (←v.mapM f)) := by simp
 
-def liftTermElabM {α} (m : TermElabM α) : SimpM α := liftM m.run'
+-- def liftTermElabM {α} (m : TermElabM α) : Sym.Simp.SimpM α := liftM m.run'
 
-dsimproc_decl _root_.Vector.mapM_mk_eq_append (_root_.Vector.mapM _ _) := fun e ↦ do
-  let_expr _root_.Vector.mapM _ _ _ _ _ f vec := e | return .continue
-  let_expr _root_.Vector.mk _ sz arr _ := vec | return .continue
-  let_expr List.toArray _ l := arr | return .continue
-  let_expr List.cons t hd tl := l | return .continue
-  let szN := (←simp sz).expr.nat?.get!
-  if szN <= 1 then return .continue
-  let hd ← liftTermElabM (mkVecLit (←mkListLit t [hd]) (mkNatLit 1))
-  let tl ← liftTermElabM (mkVecLit tl (toExpr (szN - 1)))
-  let consHdTl ← mkAppM ``HAppend.hAppend #[hd, tl]
-  let mapM ← mkAppM ``_root_.Vector.mapM #[f, consHdTl]  
-  let consMapM ← mapM.runTactic (←`(tactic| rw[$(mkIdent ``Vector.mapM_mk_singleton_append):ident]))
-  return .visit consMapM
+-- /--
+-- 0. Only for `Vector.mapM f xs`.
+-- 1. Vector.mapM f #v[a, b, c] → Vector.mapM f (#v[a] ++ #v[b, c])
+-- 2. Vector.mapM f (#v[x] ++ v) = do
+--      let __do_lift ← f x
+--      let __do_lift_1 ← Vector.mapM f v
+--      pure (#v[__do_lift] ++ __do_lift_1)
+-- -/
+-- dsimproc_decl _root_.Vector.mapM_mk_eq_append (_root_.Vector.mapM _ _) := fun e ↦ do
+--   let_expr _root_.Vector.mapM _ _ _ _ _ f vec := e | return .continue
+--   let_expr _root_.Vector.mk _ sz arr _ := vec | return .continue
+--   let_expr List.toArray _ l := arr | return .continue
+--   let_expr List.cons t hd tl := l | return .continue
+--   let szN := (←simp sz).expr.nat?.get!
+--   if szN <= 1 then return .continue
+--   let hd ← liftTermElabM (mkVecLit (←mkListLit t [hd]) (mkNatLit 1))
+--   let tl ← liftTermElabM (mkVecLit tl (toExpr (szN - 1)))
+--   let consHdTl ← mkAppM ``HAppend.hAppend #[hd, tl]
+--   let mapM ← mkAppM ``_root_.Vector.mapM #[f, consHdTl]  
+--   let consMapM ← mapM.runTactic (←`(tactic| rw[$(mkIdent ``Vector.mapM_mk_singleton_append):ident]))
+--   return .visit consMapM
 
-def mapM : SimpSet :=
-  SimpSet.withAllPost #[
-    ``Vector.mapM_mk_singleton_append,
+-- /--
+-- 0. Only for `Vector.mapM f xs`.
+-- 1. Vector.mapM f #v[a, b, c] → Vector.mapM f (#v[a] ++ #v[b, c])
+-- 2. Vector.mapM f (#v[x] ++ v) = do
+--      let __do_lift ← f x
+--      let __do_lift_1 ← Vector.mapM f v
+--      pure (#v[__do_lift] ++ __do_lift_1)
+-- -/
+-- def _root_.Vector.mapM_mk_eq_append : Sym.Simp.Simproc := fun e ↦ do
+--   let_expr _root_.Vector.mapM _ _ _ _ _ f vec := e | return .rfl
+--   let_expr _root_.Vector.mk _ sz arr _ := vec | return .rfl
+--   let_expr List.toArray _ l := arr | return .rfl
+--   let_expr List.cons t hd tl := l | return .rfl
+--   let sz' ← Sym.simp sz
+--   match (sz'.getResultExpr sz).nat? with
+--   | .none => throwError m!"{sz} does not simplify to ground"
+--   | .some szN =>
+--     if szN == 0 then return .rfl
+--     let hd ← liftTermElabM (mkVecLit (←mkListLit t [hd]) (mkNatLit 1))
+--     let tl ← liftTermElabM (mkVecLit tl (toExpr (szN - 1)))
+--     let consHdTl ← mkAppM ``HAppend.hAppend #[hd, tl]
+--     let mapM ← mkAppM ``_root_.Vector.mapM #[f, consHdTl]
+--     -- let consMapM ← mapM.runTactic (←`(tactic| rw [$(mkIdent ``Vector.mapM_mk_singleton_append):ident]))
+--     -- TODO: Definitely wrong, we need `Vector.mapM_mk_singleton_append` _at least_.
+--     -- return .step consMapM (←Sym.mkEqRefl e)
+--     return .step mapM (←Sym.mkEqRefl e)
+
+-- def mapM : SimpSet :=
+--   SimpSet.withAllPost #[
+--     ``Vector.mapM_mk_singleton_append,
     
-    ``Vector.mapM_mk_eq_append, ``Vector.mapM_singleton, ``map_pure
+--     ``Vector.mapM_mk_eq_append, ``Vector.mapM_mk_empty
+
+--     -- ``map_pure, ``Option.map_eq_map, ``Option.map_some, ``Option.bind_eq_bind
+--   ] ∪ append ∪ getElem
+
+end Vector
+
+end
+
+end CompileSets
+
+/--
+YEEEEEHAAAAAAAAW, you rootin' tootin' cowboy.
+-/
+def cowboyCast (e : Expr) (yourDeepestDesire : ℕ) : Sym.SymM Expr := do
+  let t ← Sym.inferType e
+  let_expr Vector t sz := t | throwError m!"Not a true cowboy."
+  let proof ← mkEq t (←mkAppM ``Vector #[t, mkNatLit yourDeepestDesire])
+  let e' ← e.rewriteType (←mkSorry proof false)
+  logInfo m!"Cowboy cast:\n{e}\n==>\n{e'}"
+  return e'
+  
+
+namespace SymSets
+
+section
+
+open Sym.Simp Sym
+
+def simproc? (name : Name) : MetaM (Option ConstantInfo) := do
+  let .some ci := (←getEnv).find? name | throwError m!"Undeclared constant: {name}"
+  return if ci.type.isConstOf `Lean.Meta.Sym.Simp.Simproc
+         then .some ci
+         else .none
+
+def isSimproc (name : Name) : MetaM Bool := return (←simproc? name).isSome
+
+def getSimproc (name : Name) : MetaM Sym.Simp.Simproc := do
+  discard (isSimproc name)
+  let .ok sproc := unsafe (←getEnv).evalConst Sym.Simp.Simproc {} name
+    | throwError m!"Failed to evaluate: {name}"
+  return sproc
+
+def orElse (names : Array Name) : MetaM Sym.Simp.Simproc := do
+  let simprocs ← names.mapM getSimproc
+  return simprocs.foldl (· <|> ·) (fun _ ↦ return .rfl) -- I hope this is the `.continue`...
+
+def andThen (names : Array Name) : MetaM Sym.Simp.Simproc := do
+  let simprocs ← names.mapM getSimproc
+  return simprocs.foldl (· >> ·) (fun _ ↦ return .rfl) -- I hope this is the `.continue`...
+
+def mkPostMethods (declNames : Array Name)
+                  (d : Discharger := Sym.Simp.dischargeSimpSelf) : MetaM Methods := do
+  let (procs, thms) ← declNames.toList.partitionM (liftM ∘ isSimproc)
+  let procs ← andThen procs.toArray
+  return { post := (←mkSimprocFor thms.toArray d) >> procs }
+
+def mkPreMethods (declNames : Array Name)
+                 (d : Discharger := Sym.Simp.dischargeSimpSelf) : MetaM Methods := do
+  let (procs, thms) ← declNames.toList.partitionM (liftM ∘ isSimproc)
+  let procs ← andThen procs.toArray
+  return { pre := (←mkSimprocFor thms.toArray d) >> procs }
+
+elab "sym_simp" "[" declNamesPre:ident,* "]" "[" declNamesPost:ident,* "]" : tactic => do
+  let rewritePre ← mkPreMethods (←declNamesPre.getElems.mapM fun s ↦ realizeGlobalConstNoOverload s.raw)
+  let rewritePost ← mkPostMethods (←declNamesPost.getElems.mapM fun s ↦ realizeGlobalConstNoOverload s.raw)
+  -- let rewrite ← Sym.mkSimprocFor (← declNames.getElems.mapM fun s => realizeGlobalConstNoOverload s.raw) Sym.Simp.dischargeSimpSelf
+  -- let methods : Sym.Simp.Methods := {
+  --   pre  := Sym.Simp.simpControl >> rewritePre.pre
+  --   post := Sym.Simp.evalGround >> rewritePost.post
+  -- }
+  let methods : Sym.Simp.Methods := {
+    pre  := rewritePre.pre
+    post := rewritePost.post
+  }
+  Tactic.liftMetaTactic1 fun mvarId => Sym.SymM.run do
+    let mvarId ← Sym.preprocessMVar mvarId
+    (← Sym.simpGoal mvarId methods).toOption
+
+namespace Monad
+
+def monad : MetaM Sym.Simp.Methods :=
+  mkPostMethods #[
+    ``Option.bind_assoc, ``bind_assoc,
+    ``Option.pure_def,
+    ``Option.bind_eq_bind, ``Option.bind_fun_some, ``Option.bind_some, ``bind_pure, ``pure_bind,
+    ``Option.map_eq_map, ``Option.map_some
+  ]
+
+end Monad
+
+namespace General
+
+/--
+This is more or less `Lean.Meta.Tactic.Cbv.zetaReduce`, which seems to not be exported.
+
+In `Sym`, maybe we can choose to not `zeta` certain things without breaking `simp`?
+-/
+private def zetaReduce : Simproc := fun e ↦ do
+  let .letE _ _ value body _ := e | return .rfl
+  let new := expandLet body #[value]
+  let new ← Sym.share new
+  trace[Clap.Compile.simp.proc.zeta]
+    m!"\n{e}\n==>\n{new}"
+  return .step new (←Sym.mkEqRefl new)
+
+/--
+This is more or less `Lean.Meta.Tactic.Cbv.betaReduce`, which seems to not be exported.
+-/
+def betaReduce : Simproc := fun e ↦ do
+  let new := e.headBeta
+  let new ← Sym.share new
+  return .step new (←Sym.mkEqRefl new)
+
+def zeta : MetaM Methods := do
+  return {
+    pre := zetaReduce
+  }
+
+def beta : MetaM Methods := do
+  return {
+    pre := betaReduce
+  }
+
+private def evalGround : Simproc := fun e ↦ do
+  let e' ← Sym.Simp.evalGround {} e
+  unless isSameExpr e (e'.getResultExpr e) do
+    trace[Clap.Compile.simp.proc.evalGround]
+      m!"\n{e}\n==>\n{e'.getResultExpr e}"
+  return e'
+
+def ground : MetaM Methods := do
+  return {
+    post := evalGround
+  }
+
+def compilerSet : MetaM Sym.Simp.Methods :=
+  Sym.mkMethods #[
+    ``Option.bind_assoc, ``bind_assoc,
+    ``Option.pure_def,
+    ``Option.bind_eq_bind, ``Option.bind_fun_some, ``Option.bind_some, ``bind_pure, ``pure_bind,
+    ``Option.map_eq_map, ``Option.map_some
+  ]
+
+-- private def seemsTotallySafeInDTT : Simproc := fun e ↦ do
+--   let_expr Vector _ n := ←Sym.inferType e | return .rfl
+--   let groundSize := (←Sym.simp n (←ground)).getResultExpr n
+--   if isSameExpr n groundSize then return .rfl
+--   match groundSize.nat? with
+--   | .none => throwError m!"{groundSize} is not ground.\nTODO: Maybe this is ok."
+--   | .some groundSize =>
+--     let cowboyCast e _
+--     trace[Clap.Compile.simp.proc.seemsTotallySafeInDTT]
+--       m!"{}"
+--     return .rfl
+--   -- let e' ← Sym.Simp.evalGround {} e
+--   -- unless isSameExpr e (e'.getResultExpr e) do
+--   --   trace[Clap.Compile.simp.proc.evalGround]
+--   --     m!"\n{e}\n==>\n{e'.getResultExpr e}"
+--   -- return e'
+
+end General
+
+namespace Vector
+
+-- Essentially `Vector.mk_append_mk`.
+private def mk_append_mk' : Simproc := fun e ↦ do
+  let_expr HAppend.hAppend _ _ _ _ xs ys := e | return .rfl
+  let_expr Vector t szXs := ←Sym.inferType xs | return .rfl
+  let_expr Vector _ szYs := ←Sym.inferType ys | return .rfl
+  let_expr Vector.mk _ _ xs _ := xs | return .rfl
+  let_expr Vector.mk _ _ ys _ := ys | return .rfl
+  match szXs.nat?, szYs.nat? with
+  | .some szXs, .some szYs =>
+    -- The trick here is to enforce _syntactically_ that `szXs + szYs` for concrete values
+    -- is evaluated. `Vector.mk_append_mk` leaves `q(szXs + szYs)`.
+    let append ← mkAppM ``HAppend.hAppend #[xs, ys]
+    let szAppend := toExpr (szXs + szYs)
+    let szAppendProof ← mkSorry (←mkEq (←mkAppM ``Array.size #[append]) szAppend) false
+    let e' := mkAppN
+                (.const ``Vector.mk [←getDecLevel t])
+                #[t, szAppend, append, szAppendProof]
+    let e' ← Compiler.Simp.reducedAndSharedInc e'
+    let proof ← mkSorry (←mkEq e e') false -- Probably just `Vector.mk_append_mk` up to defeq
+    trace[Clap.Compile.simp.proc.mk_append_mk]
+      m!"\n{e}\n==>\n{e'}"
+    return .step e' proof
+  | _ , _ =>
+    -- TODO: I have a feeling this sometimes misbehaves for some reason, look into this.
+    -- Notably, when using `Vector.getElem_mk` 'directly', it simps more things than this guy?
+    -- TODO: Sharing
+    logWarning m!"{e} is an append of non-ground size (TODO: remove)"
+    let thm ← mkTheoremFromDecl ``Vector.getElem_mk
+    thm.rewrite e
+
+-- def appendDbg : Sym.Simp.Simproc := fun e ↦ do
+  
+--   let_expr Vector.mk _ _ arr _ := e | return .rfl
+--   logInfo m!"{e} makes: {arr}"
+  
+--   let thm ← mkTheoremFromDecl ``List.append_toArray
+  
+--   match ←thm.pattern.match? arr with
+--   | .none => logInfo m!"{bombEmoji} Pattern:\n{thm.pattern.pattern}"
+--   | .some arr => logInfo m!"{checkEmoji} Pattern:\n{arr.args}"
+--   match ←thm.pattern.match? (←Compiler.Simp.preprocessExpr e) with
+--   | .none => logInfo m!"{bombEmoji} Pattern:\n{thm.pattern.pattern}"
+--   | .some arr => logInfo m!"{checkEmoji} Pattern:\n{arr.args}"
+--   return .rfl
+  
+
+def append : MetaM Methods :=
+  mkPostMethods #[
+    ``Vector.mk_append_mk, ``List.append_toArray,
+
+    ``List.cons_append, ``List.nil_append, ``List.append_nil,
+
+    ``Compiler.explodeVectorAppend,
+
+    -- ``appendDbg
+  ]
+
+def explode : MetaM Methods := do
+  return {
+    post := explodeVector
+    pre  := dontExplodeVector
+  }
+
+def foldlM : MetaM Methods :=
+  mkPostMethods #[
+    ``Vector.foldlM_mk, ``List.foldlM_toArray,
+
+    ``List.foldlM_cons, ``List.foldlM_nil
+  ]
+
+def getElemDbg : Sym.Simp.Simproc := fun e ↦ do
+  logInfo m!"getElemDbg: {e}"
+  let_expr GetElem.getElem _ _ _ _ _ coll i h := e | return .rfl
+  logInfo m!"coll: {coll}\ni: {i}"
+  let_expr Vector.mk _ _ arr h := coll |
+    logInfo m!"Rejected: {coll}"
+    logInfo m!"App of: {coll.getAppFnArgs}"
+    return .rfl
+  logInfo m!"arr: {arr}"
+  logInfo m!"This is getElem on Vector.mk:\n({coll})[{i}]"
+  logInfo m!"e:\n{e}"
+  
+  let thm ← mkTheoremFromDecl ``Vector.getElem_mk
+  -- logInfo m!"thm declName: {thm.declName}"
+  -- logInfo m!"thm expr: {thm.expr}"
+  logInfo m!"thm pattern: {thm.pattern.pattern}"
+  -- logInfo m!"thm rhs: {thm.rhs}"
+  -- let thmrw ← thm.rewrite e
+  -- match thmrw with
+  -- | .rfl _ _ => logInfo m!"Rewrite failed."
+  -- | .step e' _ _ _ => logInfo m!"Success. e: {e'}"
+  -- match ←thm.pattern.unify? e with
+  -- | .none => logInfo m!"NO UNIFY"
+  -- | .some res => logInfo m!"UNIFY OK!:\n{res.args}"
+  
+  -- let esimped ← e.runTactic (←`(tactic|rw! (castMode := .all) [Nat.add_zero]))
+
+  match ← thm.pattern.match? e with
+  | .none => logInfo m!"NO MATCH:\n{e}\n=?=\n{thm.pattern.pattern}"
+  | .some e' => logInfo m!"YOU TRIGGERED SON! OK!: {e'.args}"
+
+  -- match ← thm.pattern.match? esimped with
+  -- | .none => logInfo m!"NO MATCH SIMPED:\n{esimped}\n=?=\n{thm.pattern.pattern}"
+  -- | .some e' => logInfo m!"OK!: {e'.args}\n"
+  -- match ← thm.pattern.match? ((← unfoldReducible (← instantiateMVars e))) with
+  -- | .none => logInfo m!"did not match"
+  -- | .some e => logInfo m!"OK!: {e.args}"
+
+  return .rfl
+
+-- private def getElem_t : Simproc := fun e ↦ do
+--   let_expr GetElem.getElem collT _ _ _ _ coll i h := e | return .rfl
+--   let_expr Vector _ sz := collT | return .rfl
+--   let simpedSz := (←Sym.simp sz (←General.ground)).getResultExpr sz
+--   match simpedSz.nat? with
+--   | .none => return .rfl
+--   | .some simpedSzN =>
+--     return .rfl
+--     -- if simpedSz == sz then return .rfl -- TODO: `isSameExpr`?
+--     -- let coll ← cowboyCast coll simpedSzN
+--     -- let e' := ←mkAppM ``GetElem.getElem #[coll, i]
+--     -- logInfo m!"e': {e'}"
+--     -- -- This plays loose, let's pretend this is ok for now.
+--     -- return .step e' (←mkSorry (←mkEq e e') false)
+--     -- logInfo m!"szVec: {(←Sym.simp sz (←General.ground)).getResultExpr sz}"
+--     -- logInfo m!"szVecSimped: {sz}"
+--     -- let_expr Vector.mk _ sz arr _ := coll | return .rfl
+
+--     -- logInfo m!"sz: {sz}"
+--     -- logInfo m!"simped sz: {(←Sym.simp sz).getResultExpr sz}"
+--     -- return .rfl
+
+-- /--
+-- `Vector.getElem_mk` up to reducible.
+-- Trying to be as explicit as possible for `Sym`.
+-- -/
+-- private def getElem_mk : Simproc := fun e ↦ do
+--   let_expr GetElem.getElem collT _ _ _ _ coll i h := e | return .rfl
+--   let_expr Vector _ _getElemSz := collT | return .rfl
+--   let_expr Vector.mk _ _mkSz arr _ := coll | return .rfl
+--   -- Note we are not looking at `_getElemSz` and `_mkSz`.
+--   logInfo m!"WAT {h}"
+--   let szProof ← mkLt i (←mkAppM ``Array.size #[arr])
+--   let e' ← mkAppM ``GetElem.getElem #[arr, i, ←mkSorry szProof false]
+--   trace[Clap.Compile.simp.proc.getElem_mk] m!"{e}\n==>\n{e'}"
+--   return .step e' (←mkSorry (←mkEq e e') false)
+--   -- let getElemSz := (←Sym.simp getElemSz (←General.ground)).getResultExpr getElemSz
+--   -- let mkSz := (←Sym.simp mkSz (←General.ground)).getResultExpr mkSz
+--   -- unless isSameExpr getElemSz mkSz do return .rfl
+--   -- trace[Clap.Compile.simp.proc.getElem_mk] m!""
+  -- _
+
+def getElem_mk : Sym.Simp.Simproc := fun e ↦ do
+  let_expr GetElem.getElem collT _ _ _ _ coll _ _ := e | return .rfl
+  let_expr Vector.mk _ sz arr _ := coll | return .rfl
+  let_expr Vector _ getElemSz := collT | return .rfl
+  logWarning m!"Doing.\nGetElem={getElemSz}\nVec.mk={sz}"
+  if isSameExpr getElemSz sz then -- `1 + 1 ≠ 2`
+    let thm ← mkTheoremFromDecl ``Vector.getElem_mk -- TODO: Don't do this lazily here.
+    let e' ← thm.rewrite e
+    trace[Clap.Compile.simp.proc.vector_getElem_mk]
+      m!"\n{e}\n==>\n{e'.getResultExpr e}"
+    return e'
+  let simpedSz := (←Sym.simp sz (←General.ground)).getResultExpr sz
+  match simpedSz.nat? with
+  | .none =>
+    throwError m!"{simpedSz} is not ground.\nMaybe this is ok."
+    return .rfl
+  | .some simpedSzN =>
+    logInfo m!"sz:{sz}\nsimpedSz: {(←Sym.simp sz (←General.ground)).getResultExpr sz}"
+    let e' ← inferVectorProof (←mkAppM ``GetElem.getElem #[arr, mkNatLit simpedSzN])
+    let e' ← Compiler.Simp.reducedAndSharedInc e'
+    trace[Clap.Compile.simp.proc.vector_getElem_mk]
+      m!"\n{e}\n==>\n{e'}\nCheating.\nIn {collT} we pretend that {getElemSz} = {simpedSzN}."
+    return .step e' (←mkSorry (←mkEq e e') false)
+
+#check Vector.append
+#check GetElem.getElem (coll := Vector ℕ 4) (Vector.mk (n := 2 + 2) #[1, 2, 3, 4] rfl) 0 (by decide)
+def getElem : MetaM Methods :=
+  mkPostMethods #[
+    -- ``getElem_t,
+    ``Vector.getElem_mk, ``List.getElem_toArray,
+
+    ``List.getElem_cons_zero, ``List.getElem_cons_succ,
+
+    -- ``getElemDbg
+  ]
+
+def mapDbg : Sym.Simp.Simproc := fun e ↦ do
+  let_expr Array.map _ _ _ _ := e | return .rfl
+  logInfo m!"Is Array.map:\n{e}"
+  let thm ← mkTheoremFromDecl ``List.map_toArray
+  match ←thm.pattern.match? e with
+  | .none => logInfo m!"{bombEmoji} Pattern:\n{thm.pattern.pattern}"
+  | .some e => logInfo m!"{checkEmoji} Pattern:\n{e.args}"
+  match ←thm.pattern.match? (←Compiler.Simp.preprocessExpr e) with
+  | .none => logInfo m!"{bombEmoji} Pattern:\n{thm.pattern.pattern}"
+  | .some e => logInfo m!"{checkEmoji} Pattern:\n{e.args}"
+  return .rfl
+
+def map : MetaM Methods :=
+  mkPostMethods #[
+    ``Vector.map_mk, ``List.map_toArray,
+    
+    ``List.map_cons, ``List.map_nil,
+
+    ``Compiler.explodeVectorMap,
+    
+    -- ``mapDbg
+  ] ∪ mapOptim
+  where
+    mapOptim : MetaM Methods := mkPreMethods #[``List.map_id]
+
+/--
+0. Only for `Vector.mapM f xs`.
+1. Vector.mapM f #v[a, b, c] → Vector.mapM f (#v[a] ++ #v[b, c])
+2. Vector.mapM f (#v[x] ++ v) = do
+     let __do_lift ← f x
+     let __do_lift_1 ← Vector.mapM f v
+     pure (#v[__do_lift] ++ __do_lift_1)
+-/
+def _root_.Vector.mapM_mk_eq_append : Sym.Simp.Simproc := fun e ↦ do
+  -- logInfo m!"Nodes: {←e.numObjs}"
+  -- let α ← IO.monoMsNow
+  let_expr _root_.Vector.mapM _ _ _ _ _ f vec := e | return .rfl
+  let_expr _root_.Vector.mk _ sz arr _ := vec | return .rfl
+  unless arr.isAppOf ``List.toArray || arr.isAppOf ``Array.mk do return .rfl
+  let l ← arr.getAppArgs[1]?.getDM (unreachable!)
+  let_expr List.cons t hd tl := l | return .rfl
+  let sz' ← Sym.simp sz
+  match (sz'.getResultExpr sz).nat? with
+  | .none => throwError m!"{sz} does not simplify to ground. Expr:\n{e}"
+  | .some szN =>
+    if szN == 0 then return .rfl
+    let hdVec ← mkVecLit (←mkListLit t [hd]) (mkNatLit 1)
+    let tl ← mkVecLit tl (toExpr (szN - 1)) -- Doing `-1` feels scary
+    -- -- `let appendHdTl ← mkAppM ``HAppend.hAppend #[hdVec, tl]` makes a silly `k + 0` vector
+    -- TODO: This is just a WIP-test solution, it's clearly terrible.
+    let appendHdTl ← if szN == 1 then pure hdVec else mkAppM ``HAppend.hAppend #[hdVec, tl]
+    let_expr Vector _ szAppendHdTl := ←Sym.inferType appendHdTl | unreachable!
+    let szAppendHdTlQ : Q(ℕ) := szAppendHdTl
+    let szDesired : Q(ℕ) := toExpr szN
+    let proof ← mkSorry q($szAppendHdTlQ = $szDesired) false
+    logInfo m!"will try to cowboy cast: {appendHdTl}"
+    -- let thatGuy ← cowboyCast appendHdTl szN
+    let thatGuy := appendHdTl
+    let thisGuy := appendHdTl
+    let thisGuy := thatGuy
+    let mapM ← mkAppM ``_root_.Vector.mapM #[f, thisGuy]
+    let theMiddleBit ←
+      if szN == 1
+      then mkVecLit (←mkListLit t [.bvar 1]) (mkNatLit 1)
+      else pure <| mkAppN
+            (.const ``HAppend.hAppend [
+              ←getDecLevel (←Sym.inferType hdVec),
+              ←getDecLevel (←Sym.inferType tl),
+              ←getDecLevel (←Sym.inferType thisGuy)
+            ]) #[
+              ←Sym.inferType hdVec,
+              ←Sym.inferType tl,
+              ←Sym.inferType thisGuy,
+              -- ←Sym.inferType appendHdTl,
+              ←Sym.synthInstance (←mkAppM ``HAppend #[←Sym.inferType hdVec,←Sym.inferType tl,←Sym.inferType thisGuy,]),
+              ←mkVecLit (←mkListLit t [.bvar 1]) (mkNatLit 1),
+              .bvar 0
+            ]
+    let consMapM ←
+      mkAppM ``Option.bind #[
+        f.beta #[hd],
+        -- Expr.app f hdVec,
+        .lam `fst t
+          (←mkAppM ``Option.bind #[
+                     ←mkAppM ``Vector.mapM #[f, tl],
+                     .lam `snd (←Sym.inferType tl)
+                       (←mkAppM ``Option.some #[theMiddleBit])
+                       .default
+          ])
+          .default 
+      ]
+
+    trace[Clap.Compile.simp.proc.vector_mapM_mk_eq_append]
+      m!"\n{e}\n==>\n{consMapM}"
+    -- let ω ← IO.monoMsNow
+    -- logInfo m!"timing: {Float.ofNat (ω - α)/Float.ofNat 1000}"
+    -- logInfo m!"Nodes: {←consMapM.numObjs}"
+    let consMapM ← Compiler.Simp.reducedAndSharedInc consMapM
+    return .step consMapM (←mkSorry (←mkEq e mapM) false)
+    
+    -- -- TODO: I am guessing this is... slow?
+    -- let consMapM ← mapM.runTactic (←`(tactic| rw[$(mkIdent ``Vector.mapM_mk_singleton_append):ident]))
+    -- -- TODO: Puh-ROOF!
+    -- return .step consMapM (←mkSorry (←mkEq e mapM) false)
+
+/--
+`Vector.mapM_mk_singleton_append` is a part of `Vector.mapM_mk_append` to ensure that
+the transformation `#v[a, b] ==> #v[a] ++ #v[b]` does not get undone by `Vector.mk_append_mk`.
+-/
+def mapM : MetaM Methods :=
+  mkPostMethods #[
+    ``Vector.mapM_mk_eq_append, ``Vector.mapM_nil,
+
+    ``Compiler.explodeVectorMapM
   ] ∪ append ∪ getElem
 
 end Vector
 
-end CompileSets
+end
 
-namespace Exampru
+end SymSets
 
-def compileExample (ex : Name) (simpset : SimpSet) (only : Bool := true) : TermElabM Format := do
-  compile (((←getEnv).find? ex).get!.value!) simpset only >>= (liftM ∘ PrettyPrinter.ppExpr)
+def compileExample (ex : Name) (simpset : Sym.Simp.Methods) : Sym.Simp.SimpM Format := do
+  compile (((←getEnv).find? ex).get!.value!) simpset >>= (liftM ∘ PrettyPrinter.ppExpr)
+
+def compileJustSym (e : Expr) (simpset : Sym.Simp.Methods) : Sym.Simp.SimpM Format := do
+  lambdaTelescope e fun args e ↦ do
+    let compiled ← Compiler.Simp.simplify (simpset ∪ (←SymSets.General.compilerSet)) e
+    logInfo m!"Compiled: {compiled}"
+    Sym.mkLambdaFVarsS args compiled >>= (liftM ∘ PrettyPrinter.ppExpr)
+
+def compileExampleJustSym (ex : Name) (simpset : Sym.Simp.Methods) : Sym.Simp.SimpM Format := do
+  let e := ((←getEnv).find? ex).get!.value!
+  compileJustSym e simpset
+
+open SymSets in
+elab "compile_just_sym" "[" simps:ident,* "]" : tactic => do
+  let simps ← simps.getElems.mapM fun s ↦ realizeGlobalConstNoOverload s.raw
+  let methods ← simps.mapM (liftM ∘ Simp.API.getMethodsM)
+  let methods ← liftM <| methods.foldl (fun method acc ↦ method ∪ acc) (pure {})
+  Tactic.liftMetaTactic1 fun mvarId => Sym.SymM.run do
+    let mvarId ← Sym.preprocessMVar mvarId
+    (← Sym.simpGoal mvarId methods).toOption
 
 def eq0 (e : Nat) : Option Unit := .some ()
+
+def spoon (m : Sym.Simp.SimpM Format) : MetaM Format :=
+  m.run' {} |>.run
+
+namespace ExampruSym
+
+open SymSets Monad General Vector
+
+def ex₀ : Option Unit := do
+  eq0 0
+  eq0 1
+  let _res ← ([0, 1].foldlM (init := ()) fun _ _ ↦ eq0 2)
+  eq0 3
+  return ()
+
+/--
+info: (eq0 0).bind fun x =>
+  (eq0 1).bind fun x =>
+    ((eq0 2).bind fun init => (eq0 2).bind fun init => pure init).bind fun _res => (eq0 3).bind fun x => pure PUnit.unit
+-/
+#guard_msgs in
+#eval spoon <| do compileExample ``ex₀ (←foldlM)
+
+def ex₁ (_vec : Vector Nat 3) : Option Unit := do
+  eq0 #v[4, 5][0]
+
+set_option profiler true
+set_option profiler.threshold 10
+
+
+-- /-- info: fun _vec => eq0 4 -/
+-- #guard_msgs in
+#eval spoon <| do compileExampleJustSym ``ex₁ (←getElem)
+set_option trace.Clap.Compile true
+
+def ex₂ (vec : Vector Nat 3) : Option Unit := do
+  let x := (vec ++ vec)[0] -- `GetElem (Vector _ (3 + 3))`
+  eq0 x
+
+/-- info: fun vec => eq0 vec[0] -/
+#guard_msgs in
+#eval spoon <| do compileExampleJustSym ``ex₂ (←(append ∪ zeta ∪ getElem))
+
+def ex₃ (vec : Vector Nat 200) : Option Unit := do
+  let x := vec.map (·+1)
+  eq0 x[0]
+-- set_option maxRecDepth 1000
+/-- info: fun vec => eq0 (vec[0] + 1) -/
+#guard_msgs in
+#eval spoon <| do compileExampleJustSym ``ex₃ (←(map ∪ zeta ∪ getElem))
+
+def ex₄ (vec : Vector Nat 2) : Option Unit := do
+  let x ← vec.mapM (fun x ↦ return x + 1)
+  eq0 x[0]
+-- set_option trace.Clap.Compile true
+
+set_option profiler true
+-- set_option trace.sym.issues true
+-- /-- info: fun vec => eq0 (vec[0] + 1) -/
+
+set_option trace.Clap.Compile.debug.simp true
+set_option pp.exprSizes true
+-- set_option debug.skipKernelTC true in
+#eval spoon <| do compileExampleJustSym ``ex₄ (←(ground ∪ mapM ∪ getElem ∪ zeta))
+
+example {vec : Vector Nat 2} : ex₄ vec = sorry := by
+  unfold ex₄
+  compile_just_sym [ground, SymSets.Vector.mapM, SymSets.Vector.getElem, zeta, compilerSet]
+
+#exit
+
+example {vec : Vector Nat 1} : ex₄ vec = sorry := by
+  unfold ex₄
+  rcases vec with ⟨arr, h⟩
+  rcases arr with ⟨l⟩
+  rcases l with _ | ⟨hd, _ | ⟨_, _⟩⟩
+  simp at h
+  sym_simp [] [Option.pure_def, mapM_singleton, Option.bind_eq_bind, Option.bind_some, getElem_mk,
+    List.getElem_toArray, List.getElem_cons_zero]
+  
+
+
+example {vec : Vector Nat 1} : eq0
+  (Vector.mk (n := 1 + 0) { toList := [vec[0] + 1] } (Eq.trans (List.append_toArray [vec[0] + 1] []) (congrArg Array.mk (List.append_nil [vec[0] + 1])) ▸
+  mk_append_mk._proof_1 rfl (of_eq_true (Eq.trans (congrFun' (congrArg Eq List.size_toArray) 0) (eq_self 0))) : (fun toArray : Array _ => toArray.size = 1 + 0) { toList := [vec[0] + 1] }))[0] = sorry := by
+  -- rw [getElem_mk]
+  sym_simp [] [getElem_mk, List.getElem_toArray, List.getElem_cons_zero]
+  
+  done
+
+  
+  
+  
+  -- sym_simp [dontExplodeVector] [explodeVector, Vector.mapM_mk_eq_append]
+  -- sym_simp [] [Vector.mapM_singleton, Vector.mapM_mk_singleton_append]
+  
+  
+  
+
+  simp only [Nat.reduceAdd, Option.pure_def, Option.bind_eq_bind, Option.bind_some, getElem_mk,
+    List.getElem_toArray, List.getElem_cons_zero]
+
+
+  sorry
+
+-- example :
+--   #[4, 5][0] = sorry := by
+--   sym_simp [List.getElem_toArray]
+
+-- example {v : Vector Nat 3} : ex₁ v = sorry := by
+--   unfold ex₁
+--   sym_simp [Vector.getElem_mk, List.getElem_toArray]
+
+-- def getElem : MetaM Lean.Meta.Sym.Simp.Methods :=
+--   mkPostMethods #[
+--     ``List.getElem_toArray
+--   ]
+
+-- def getElem' : MetaM Lean.Meta.Sym.Simp.Methods := do
+--   let rewrite ← Sym.mkSimprocFor #[``List.getElem_toArray, ``Vector.getElem_mk] Sym.Simp.dischargeSimpSelf
+--   return {
+--     post := rewrite
+--   }
+
+-- #eval spoon <| do compileExample ``ex₁ (←getElem')
+
+end ExampruSym
+
+namespace Exampru
 
 def ex₀ : Expr := q(
   do eq0 0
@@ -255,22 +1125,18 @@ def ex₀ : Expr := q(
      eq0 3
      return ()
 )                    
-
-/--
-info: do
-  eq0 0
-  eq0 1
-  do
-    eq0 2
-    let init ← eq0 2
-    pure init
-  eq0 3
-  pure ()
--/
-#guard_msgs in
-#eval compile ex₀
-  (SimpSet.withAllPost #[``List.foldlM_cons, ``List.foldlM_nil]) >>=
-  (liftM ∘ PrettyPrinter.ppExpr)
+-- set_option trace.Clap.Compile true
+-- /--
+-- info: (eq0 0).bind fun x =>
+--   (eq0 1).bind fun x =>
+--     ((eq0 2).bind fun init => (eq0 2).bind fun init => pure init).bind fun _res => (eq0 3).bind fun x => pure ()
+-- -/
+-- #guard_msgs in
+-- #eval show MetaM _ from do
+--   let res := compile ex₀
+--     (SimpSet.withAllPost #[``List.foldlM_cons, ``List.foldlM_nil]) >>=
+--     (liftM ∘ PrettyPrinter.ppExpr)
+--   res.run' default |>.run
 
 def ex₁ (n : Nat) : Option Unit := do
   eq0 0
@@ -280,7 +1146,9 @@ def ex₁ (n : Nat) : Option Unit := do
   eq0 (res'[1])
   return ()
 
-open CompileSets Vector
+open CompileSets Vector Logic
+
+set_option trace.Clap.Compile true
 
 /--
 info: fun n => do
@@ -288,45 +1156,44 @@ info: fun n => do
   (eq0 (n + 1)).bind fun a => (eq0 7).bind fun a => some ()
 -/
 #guard_msgs in
-#eval compileExample ``ex₁
-        (foldlM ∪ getElem ∪ map ∪ explode)
+#eval spoon <| compileExample ``ex₁ (foldlM ∪ map ∪ getElem ∪ explode)
 
-def ex₂ (vec : Vector Nat 4) : Option Unit := do
-  eq0 ((vec ++ vec)[0])
-  eq0 0
-  let _res ← vec.foldlM (fun acc x ↦ do eq0 x; acc) (eq0 4)
-  eq0 4
+-- def ex₂ (vec : Vector Nat 4) : Option Unit := do
+--   eq0 ((vec ++ vec)[0])
+--   eq0 0
+--   let _res ← vec.foldlM (fun acc x ↦ do eq0 x; acc) (eq0 4)
+--   eq0 4
 
-/--
-info: fun vec => do
-  eq0 vec[0]
-  eq0 0
-  (eq0 vec[0]).bind fun a =>
-      (eq0 4).bind fun a => (eq0 vec[1]).bind fun a => (eq0 vec[2]).bind fun a => (eq0 vec[3]).bind fun a => eq0 4
--/
-#guard_msgs in
-#eval compileExample ``ex₂
-        (foldlM ∪ getElem ∪ map ∪ explode ∪ append)
+-- /--
+-- info: fun vec => do
+--   eq0 vec[0]
+--   eq0 0
+--   (eq0 vec[0]).bind fun a =>
+--       (eq0 4).bind fun a => (eq0 vec[1]).bind fun a => (eq0 vec[2]).bind fun a => (eq0 vec[3]).bind fun a => eq0 4
+-- -/
+-- #guard_msgs in
+-- #eval compileExample ``ex₂
+--         (foldlM ∪ getElem ∪ map ∪ explode ∪ append)
 
-def ex₃ (vec : Vector Nat 3) : Option Unit := do
-  eq0 ((vec ++ vec)[0])
-  eq0 0
-  let res := vec.mapIdx fun i _ ↦ i
-  eq0 res[0]
-  eq0 res[1]
-  eq0 res[2]
+-- def ex₃ (vec : Vector Nat 3) : Option Unit := do
+--   eq0 ((vec ++ vec)[0])
+--   eq0 0
+--   let res := vec.mapIdx fun i _ ↦ i
+--   eq0 res[0]
+--   eq0 res[1]
+--   eq0 res[2]
 
-/--
-info: fun vec => do
-  eq0 vec[0]
-  eq0 0
-  eq0 0
-  eq0 1
-  eq0 2
--/
-#guard_msgs in
-#eval compileExample ``ex₃
-        (foldlM ∪ getElem ∪ map ∪ explode ∪ append ∪ mapIdx)
+-- /--
+-- info: fun vec => do
+--   eq0 vec[0]
+--   eq0 0
+--   eq0 0
+--   eq0 1
+--   eq0 2
+-- -/
+-- #guard_msgs in
+-- #eval compileExample ``ex₃
+--         (foldlM ∪ getElem ∪ map ∪ explode ∪ append ∪ mapIdx)
 
 def ex₄ (vec : Vector Nat 3) : Option Unit := do
   eq0 ((vec ++ vec)[0])
@@ -345,56 +1212,94 @@ info: fun vec => do
   eq0 (2 * vec[2] + 1)
 -/
 #guard_msgs in
-#eval compileExample ``ex₄
+#eval spoon <| compileExample ``ex₄
         (foldlM ∪ getElem ∪ map ∪ explode ∪ append ∪ mapIdx ∪ zipWith)
   
-def ex₅ (vec : Vector Nat 3) : Option Unit := do
-  eq0 ((vec ++ vec)[0])
-  eq0 0
-  let res := (vec.drop 1).take 1
-  eq0 res[0]
+-- def ex₅ (vec : Vector Nat 3) : Option Unit := do
+--   eq0 ((vec ++ vec)[0])
+--   eq0 0
+--   let res := (vec.drop 1).take 1
+--   eq0 res[0]
 
-/--
-info: fun vec => do
-  eq0 vec[0]
-  eq0 0
-  eq0 vec[1]
--/
-#guard_msgs in
-#eval compileExample ``ex₅
-        (foldlM ∪ getElem ∪ map ∪ explode ∪ append ∪ mapIdx ∪ zipWith ∪ take ∪ drop)
+-- /--
+-- info: fun vec => do
+--   eq0 vec[0]
+--   eq0 0
+--   eq0 vec[1]
+-- -/
+-- #guard_msgs in
+-- #eval compileExample ``ex₅
+--         (foldlM ∪ getElem ∪ map ∪ explode ∪ append ∪ mapIdx ∪ zipWith ∪ take ∪ drop)
 
-def ex₆ (vec : Vector Nat 3) : Option Unit := do
-  eq0 ((vec ++ vec)[0])
-  eq0 0
-  let res := vec.sum
-  eq0 res
+-- def ex₆ (vec : Vector Nat 3) : Option Unit := do
+--   eq0 ((vec ++ vec)[0])
+--   eq0 0
+--   let res := vec.sum
+--   eq0 res
 
-/--
-info: fun vec => do
-  eq0 vec[0]
-  eq0 0
-  eq0 (vec[0] + vec[1] + vec[2])
--/
-#guard_msgs in
-#eval compileExample ``ex₆
-        (foldlM ∪ getElem ∪ map ∪ explode ∪ append ∪ mapIdx ∪ zipWith ∪ take ∪ drop ∪ sum)
+-- /--
+-- info: fun vec => do
+--   eq0 vec[0]
+--   eq0 0
+--   eq0 (vec[0] + vec[1] + vec[2])
+-- -/
+-- #guard_msgs in
+-- #eval compileExample ``ex₆
+--         (explode ∪ append  ∪ sum)
 
-def ex₇ (vec : Vector Nat 3) : Option Unit := do
-  let vec := vec.zipWith (·+·) #v[1, 5, 10]
-  eq0 42
-  let res ← vec.mapM (fun n ↦ return n + 1)
-  eq0 res[0]
-  eq0 res[1]
-  eq0 res[2]
+-- def ex₇ (vec : Vector Nat 3) : Option Unit := do
+--   let vec := vec.zipWith (·+·) #v[1, 5, 10]
+--   eq0 42
+--   let res ← vec.mapM (fun n ↦ return n + 1)
+--   eq0 res[0]
+--   eq0 res[1]
+--   eq0 res[2]
 
-/--
-info: fun vec => do
-  eq0 42
-  (eq0 (vec[0] + 2)).bind fun a => (eq0 (vec[1] + 6)).bind fun a => eq0 (vec[2] + 11)
--/
-#guard_msgs in
-#eval compileExample ``ex₇ (explode ∪ mapM ∪ zipWith)
+-- example {inputs : Vector Nat 2} {sigma : ℕ → Option Unit} :
+--   Vector.mapM sigma
+--       #v[0 + 6745197990210204598374042828761989596302876299545964402857411729872131034734,
+--         inputs[0] + 426281677759936592021316809065178817848084678679510574715894138690250139748,
+--         inputs[1] + 4014188762916583598888942667424965430287497824629657219807941460227372577781] =
+--   sorry := by
+--   simp +singlePass [Vector.mapM_mk_eq_append]
+--   simp +singlePass [Vector.mapM_mk_eq_append]
+--   simp? +singlePass [Vector.mapM_mk_eq_append]
+--   done
+
+-- def ex₈ (vec : Vector Nat 3) : Option Unit := do
+--   let res := (#v[0] ++ vec).extract 1 2
+--   eq0 res[0]
+
+-- #eval compileExample ``ex₈ (append ∪ explode ∪ extract ∪ getElem)
+
+
+-- def ex₉ (vec : Vector Nat 3) : Option Unit := do
+--   let res := (#v[0] ++ vec).set 0 42
+--   eq0 res[0]
+
+-- #eval compileExample ``ex₉ (append ∪ explode ∪ extract ∪ getElem ∪ set)
+#check Sym.simp
+opaque share : Nat → Option Nat
+
+-- example {inputs : Vector Nat 3} : ((share ((0 + 66) * (0 + 66))).bind fun a =>
+--   (share (a * a)).bind fun a =>
+--     (share ((inputs[0] + 66) * (inputs[0] + 66))).bind fun a_1 =>
+--       (share (a_1 * a_1)).bind fun a_2 =>
+--         (share ((inputs[1] + 66) * (inputs[1] + 66))).bind fun a_3 =>
+--           (share (a_3 * a_3)).bind fun a_4 =>
+--             some
+--               #v[66 * ([a * (0 + 66), a_2 * (inputs[0] + 66), a_4 * (inputs[1] + 66)][0] + 66) +
+--                   (66 * ([a * (0 + 66), a_2 * (inputs[0] + 66), a_4 * (inputs[1] + 66)][1] + 66) +
+--                     (66 * ([a * (0 + 66), a_2 * (inputs[0] + 66), a_4 * (inputs[1] + 66)][2] + 66) + 0)),
+--                 66 * ([a * (0 + 66), a_2 * (inputs[0] + 66), a_4 * (inputs[1] + 66)][0] + 66) +
+--                   (66 * ([a * (0 + 66), a_2 * (inputs[0] + 66), a_4 * (inputs[1] + 66)][1] + 66) +
+--                     (66 * ([a * (0 + 66), a_2 * (inputs[0] + 66), a_4 * (inputs[1] + 66)][2] + 66) + 0)),
+--                 66 * ([a * (0 + 66), a_2 * (inputs[0] + 66), a_4 * (inputs[1] + 66)][0] + 66) +
+--                   (66 * ([a * (0 + 66), a_2 * (inputs[0] + 66), a_4 * (inputs[1] + 66)][1] + 66) +
+--                     (66 * ([a * (0 + 66), a_2 * (inputs[0] + 66), a_4 * (inputs[1] + 66)][2] + 66) + 0))]) = sorry := by
+--   simp?
+--   sorry
+--   done
 
 end Exampru
 
