Clap/Compiler/Simp.lean
@@ -1,4 +1,5 @@
 import Lean
+import Lean.Meta.Sym.SymM
 
 open Lean Meta Elab
 
@@ -59,6 +60,101 @@ def SimpSet.union (s₁ s₂ : SimpSet) : SimpSet where
   pos := s₁.pos ++ s₂.pos
   neg := s₁.neg ++ s₂.neg
 
+-- open Sym.Simp in
+-- public def mkSimprocFor (declNames : Array Name) (d : Discharger := dischargeNone) : MetaM Simproc := do
+--   let mut thms : Theorems := {}
+--   for declName in declNames do
+--     thms := thms.insert (← mkTheoremFromDecl declName)
+--   return thms.rewrite d
+
+-- def mkAlternativeSimprocFor (name : Name) : MetaM Sym.Simp.Simproc := do
+--   let thm := Sym.Simp.mkTheoremFromDecl name
+--   _
+
+def ciOfName (name type : Name) : MetaM (Option ConstantInfo) := do
+  let .some ci := (←getEnv).find? name | throwError m!"Undeclared constant: {name}"
+  return if ci.type.isConstOf type
+         then .some ci
+         else .none
+
+def simproc? (name : Name) : MetaM (Option ConstantInfo) := do
+  ciOfName name `Lean.Meta.Sym.Simp.Simproc
+
+def isSimproc (name : Name) : MetaM Bool := return (←simproc? name).isSome
+
+def getSimproc (name : Name) : MetaM Sym.Simp.Simproc := do
+  guard (←isSimproc name)
+  let .ok sproc := unsafe (←getEnv).evalConst Sym.Simp.Simproc {} name
+    | throwError m!"Failed to evaluate: {name}"
+  return sproc
+
+def methods? (name : Name) : MetaM (Option ConstantInfo) := do
+  ciOfName name `Lean.Meta.Sym.Simp.Methods
+
+def isMethods (name : Name) : MetaM Bool := return (←methods? name).isSome
+
+def getMethods (name : Name) : MetaM Sym.Simp.Methods := do
+  guard (←isMethods name)
+  let .ok methods := unsafe (←getEnv).evalConst Sym.Simp.Methods {} name
+    | throwError m!"Failed to evaluate: {name}"
+  return methods
+
+def methodsM? (name : Name) : MetaM (Option ConstantInfo) := do
+  let .some ci := (←getEnv).find? name | throwError m!"Undeclared constant: {name}"
+  let (``Lean.Meta.MetaM, #[type]) := ci.type.getAppFnArgs | return .none
+  return if type.isConstOf ``Sym.Simp.Methods
+         then .some ci
+         else .none
+
+def isMethodsM (name : Name) : MetaM Bool := return (←methodsM? name).isSome
+
+def getMethodsM (name : Name) : MetaM (MetaM Sym.Simp.Methods) := do
+  guard (←isMethodsM name)
+  let .ok methods := unsafe (←getEnv).evalConst (MetaM Sym.Simp.Methods) {} name
+    | throwError m!"Failed to evaluate: {name}"
+  return methods
+
+def orElse (names : Array Name) : MetaM Sym.Simp.Simproc := do
+  let simprocs ← names.mapM getSimproc
+  return simprocs.foldl (· <|> ·) (fun _ ↦ return .rfl) -- I hope this is the `.continue`...
+
+def andThen (names : Array Name) : MetaM Sym.Simp.Simproc := do
+  let simprocs ← names.mapM getSimproc
+  return simprocs.foldl (· >> ·) (fun _ ↦ return .rfl) -- I hope this is the `.continue`...
+
+instance : Singleton Sym.Simp.Simproc Sym.Simp.Methods where
+  singleton x := {post := x}
+
+instance : Union Sym.Simp.Methods := ⟨
+  fun m₁ m₂ =>
+    {
+      pre := m₁.pre >> m₂.pre
+      post := m₁.post >> m₂.post
+    }
+  ⟩
+
+def SimpSet.toMethods (s : SimpSet) : Sym.SymM Sym.Simp.Methods := do
+  unless s.neg.isEmpty do throwError m!"Erasing Sym.simp theorems currently unsupported."
+  let (pre, post) := (s.pos.partition fun (_, order) ↦ order matches .Pre).map (·.map Prod.fst) (·.map Prod.fst)
+  let (preSimp, preThm) ← pre.toList.partitionM (liftM ∘ isSimproc)
+  let (postSimp, postThm) ← post.toList.partitionM (liftM ∘ isSimproc)
+  logInfo m!"preThm: {preThm}\npreSimp: {preSimp}\npostThm:{postThm}\npostSimp:{postSimp}"
+  let simprocsPre := (←Sym.mkSimprocFor preThm.toArray) <|> (←andThen preSimp.toArray)
+  let simprocsPost := (← Sym.mkSimprocFor postThm.toArray) <|> (←andThen postSimp.toArray)
+  return {
+    pre := simprocsPre
+    post := simprocsPost
+  }
+
+def config : Sym.Simp.Config :=
+  {
+    maxSteps := 1_000_000
+  }
+
+section Debug
+deriving instance Repr for Sym.Simp.Config
+end Debug
+
 instance : Union SimpSet := ⟨SimpSet.union⟩
 
 instance : Singleton Name SimpSet where
@@ -69,7 +165,7 @@ section
 open Parser Tactic
 
 set_option hygiene false in
-def configStx (singlePass : Bool := false) : MetaM (TSyntax ``optConfig) := do
+def configStx (singlePass : Bool := false) : Sym.Simp.SimpM (TSyntax ``optConfig) := do
   `(optConfig|(
       config := {
         failIfUnchanged := false
@@ -81,7 +177,7 @@ def configStx (singlePass : Bool := false) : MetaM (TSyntax ``optConfig) := do
   where defaultMaxSteps := 10_000_000
 
 def simpSetStx (sets : Array Lemma) :
-  MetaM (Syntax.TSepArray [``simpStar, ``simpErase, ``simpLemma] ",") := do
+  Sym.Simp.SimpM (Syntax.TSepArray [``simpStar, ``simpErase, ``simpLemma] ",") := do
   let arrStx ← sets.mapM fun lemma ↦
     match lemma with
     | .neg name => `(simpErase|-$(mkIdent name):term)
@@ -94,19 +190,42 @@ end API
 
 open API
 
+open Sym in
+def preprocessExpr (e : Expr) : SymM Expr := do
+  shareCommon (←unfoldReducible (←instantiateMVars e))
+
+open Sym in
+def reducedAndSharedInc (e : Expr) : SymM Expr := do
+  shareCommonInc (←unfoldReducible e)
+
 set_option hygiene false in
 def mkSimp (simpset : SimpSet)
-           (only singlePass : Bool := false) : TermElabM (TSyntax `tactic) := do
+           (only singlePass : Bool := false) : Sym.Simp.SimpM (TSyntax `tactic) := do
   let simpsetStx ← simpSetStx simpset.toSimpSet
   if only
   then `(tactic| simp $(←configStx singlePass) only [$[$simpsetStx],*])
   else `(tactic| simp $(←configStx singlePass) [$[$simpsetStx],*])
 
+def forceHeartbeats {α : Type} {m : Type → Type} [MonadWithReaderOf Core.Context m]
+                    (heartBeats : Nat) : m α → m α :=
+  withTheReader Core.Context ({· with maxHeartbeats := heartBeats * 1000})
+
 set_option hygiene false in
-def simplify (simpset : SimpSet) (e : Expr) (only singlePass : Bool := false) : TermElabM Expr := do
-  lambdaTelescope e fun args body ↦ do
-    body.runTactic (←mkSimp simpset only singlePass) >>= liftM ∘ mkLambdaFVars args
-  where simpAll := `simpAll
+def simplify (simpset : Sym.Simp.Methods) (e : Expr) : Sym.Simp.SimpM Expr := do
+  let e ← preprocessExpr e
+  tryCatchRuntimeEx
+    do return (←Sym.simp e simpset config).getResultExpr e
+    fun exc =>
+      throwError m!"***SIMP ERRROR***\nExpression:\n{e}\nInternal:\n{exc.toMessageData}"
+
+  -- lambdaTelescope e fun args body ↦ do
+  --   logInfo m!"Calling Sym.simp on:\n{body}\ncfg:{repr config}"
+  --   let res ← Sym.simp body simpset config
+  --   match res with
+  --   | .rfl e _ => logInfo m!"rfl"
+  --   | .step e prf _ _ => logInfo m!"step[e]:\n{e}\nstep[prf]:\n{prf}"
+  --   logInfo m!"Result:\n{res.getResultExpr body}"
+  --   Sym.mkLambdaFVarsS args (res.getResultExpr body)
 
 end Simp
 
