Clap/Compiler/Vectors.lean
@@ -1,3 +1,4 @@
+import Clap.Compiler.Simp
 import Clap.Compiler.Wheels
 import Qq
 import Mathlib.Tactic
@@ -8,66 +9,244 @@ open Lean Meta Elab Qq
 
 namespace Clap.Compiler
 
-def getElemVectorOfIdx (coll : Expr) (idx : Nat) : TermElabM Expr := do
-  let_expr Vector _ sz := ← Meta.inferType coll | throwError m!"{coll} must be a Vector."
+-- def getElemVectorOfIdx (coll : Expr) (len idx : Nat) : Sym.Simp.SimpM Expr := do
+--   let idxQ : Q(Nat) := ToExpr.toExpr idx
+--   let szQ : Q(Nat) := mkNatLit len
+--   let getElemSansProof ← Meta.mkAppM ``GetElem.getElem #[coll, idxQ]
+--   let proof ← Sym.Simp.liftTermElabM (
+--                 Elab.Term.mkTacticMVar q($idxQ < $szQ) (←`(by get_elem_tactic)) .term
+--               )
+--   Sym.Simp.liftTermElabM Term.synthesizeSyntheticMVarsNoPostponing
+--   instantiateMVars <| mkAppN getElemSansProof #[proof]
+
+-- def inferVectorProof (vectorSansProof : Expr) : Sym.Simp.SimpM Expr := do
+--   let .forallE _ argT _ _ ← inferType vectorSansProof | unreachable!
+--   let proof ← Sym.Simp.liftTermElabM (Term.mkTacticMVar argT (←`(by simp)) .term)
+--   Sym.Simp.liftTermElabM Term.synthesizeSyntheticMVarsNoPostponing
+--   pure (Expr.app vectorSansProof proof) >>= instantiateMVars
+
+def getElemVectorOfIdx (coll : Expr) (len idx : Nat) : Sym.Simp.SimpM Expr := do
   let idxQ : Q(Nat) := ToExpr.toExpr idx
-  let szQ : Q(Nat) := sz
-  let getElemSansProof ← Meta.mkAppM ``GetElem.getElem #[coll, ToExpr.toExpr idx]
-  let proof ← Elab.Term.mkTacticMVar q($idxQ < $szQ) (←`(by get_elem_tactic)) .term
-  Term.synthesizeSyntheticMVarsNoPostponing
-  instantiateMVars <| mkAppN getElemSansProof #[proof]
+  let szQ : Q(Nat) := mkNatLit len
+  let getElemSansProof ← Meta.mkAppM ``GetElem.getElem #[coll, idxQ]
+  return mkAppN getElemSansProof #[←mkSorry q($idxQ < $szQ) false]
 
-def inferVectorProof (vectorSansProof : Expr) : TermElabM Expr := do
+def inferVectorProof (vectorSansProof : Expr) : Sym.Simp.SimpM Expr := do
   let .forallE _ argT _ _ ← inferType vectorSansProof | unreachable!
-  let proof ← Term.mkTacticMVar argT (←`(by simp)) .term
-  Term.synthesizeSyntheticMVarsNoPostponing
-  pure (Expr.app vectorSansProof proof) >>= instantiateMVars
+  -- logInfo m!"vectorSansProof: {vectorSansProof}\ntype: {←inferType vectorSansProof}"
+  pure (Expr.app vectorSansProof (←mkSorry argT false)) -- >>= instantiateMVars
 
-def mkVecLit (l : Expr) (sz : Expr) : TermElabM Expr := do
-  -- logInfo m!"mkVecLit:\n{l}\nsz:\n{sz}"
+def mkVecLit (l : Expr) (sz : Expr) : Sym.Simp.SimpM Expr := do
   let array ← mkAppM ``List.toArray #[l]
   let t := (←inferType array).getAppArgs[0]!
   let u ← getDecLevel t
   let vectorSansProof := mkAppN (.const ``_root_.Vector.mk [u]) #[t, sz, array]
-  inferVectorProof vectorSansProof
-
-def sequenceAsVecExpr (name : Expr) (t : Expr) (len : Nat) : TermElabM Expr := do
-  let array ← mkAppM ``List.toArray #[
-    ←mkListLit t (←List.range len |>.mapM (getElemVectorOfIdx name))
-  ]
-  let u ← getDecLevel t
-  inferVectorProof (mkAppN (.const ``Vector.mk [u]) #[t, toExpr len, array])
-
-def needsExploding (e : Expr) : SimpM Bool := do
-  let t ← inferType e
-  return t.isAppOf ``Vector
+  let vector ← inferVectorProof vectorSansProof
+  return vector
 
 /--
-Intended as `↑` in combination with `↓dontExplodeVector`.
+TODO: Use mkVecLit
 -/
-dsimproc_decl explodeVector (_) := fun e ↦ do
-  let t ← inferType e
-  let_expr Vector t sz := t | return .continue
-  
-  if e.isFVar && (←needsExploding e)
-  then let explodedVec ← (sequenceAsVecExpr e t (←Simp.simp sz).1.nat?.get!).run'
-       trace[Clap.Compile.simp.kaboom] m!"Exploding:\n{e}\n==>\n{explodedVec}"
-       return .done explodedVec
-  else return .continue
+def sequenceAsVecExpr (name : Expr) (t : Expr) (len : Nat) : Sym.Simp.SimpM Expr := do
+  let e' ← mkVecLit
+             (←mkListLit t (←List.range len |>.mapM (getElemVectorOfIdx name len)))
+             (mkNatLit len)
+  trace[Clap.Compile.simp.proc.sequenceAsVecExpr]
+    m!"\n{name}[length = {len}][elemType = {t}]\n==>\n{e'}"
+  Sym.shareCommonInc e'
 
-def rejectVectorSansProof (coll e : Expr) : SimpM Simp.DStep := do
-  let_expr Vector _ _ := ← inferType coll | return .continue
-  return .done e
+-- def needsExploding (e : Expr) : SimpM Bool := do
+--   let t ← inferType e
+--   return t.isAppOf ``Vector
+
+lemma abc {α} {vec : Vector α 2} : vec = #v[vec[0], vec[1]] := by
+  rcases vec with ⟨⟨_ | ⟨_, _ | ⟨_, _ | ⟨_, tl⟩⟩⟩⟩, h⟩
+  · cases h
+  · cases h
+  · rfl
+  · cases h
+
+lemma abc' : ∀ {α} {vec : Vector α 2}, vec = #v[vec[0], vec[1]] :=
+  fun {α vec} ↦
+    vec.casesOn fun arr h ↦
+      arr.casesOn
+        (motive := fun x ↦ ∀ (h : x.size = 2), Vector.mk x h = #v[(Vector.mk x h)[0], (Vector.mk x h)[1]])
+        (
+          fun l h ↦
+            l.casesOn
+              (motive := fun x =>
+                ∀ (h : {toList := x : Array _}.size = 2),
+                  Vector.mk { toList := x } h =
+                  #v[(Vector.mk { toList := x } h)[0], (Vector.mk { toList := x } h)[1]])
+              (fun h ↦ h.casesOn
+                         (motive := fun a t ↦
+                           2 = a →
+                           h ≍ t →
+                           Vector.mk { toList := [] } h =
+                           #v[(Vector.mk { toList := [] } h)[0], (Vector.mk { toList := [] } h)[1]])
+              (fun h_1 ↦ False.elim (noConfusion_of_Nat Nat.ctorIdx h_1)) rfl HEq.rfl)
+              (
+                fun head tail ↦
+                  tail.casesOn
+                    (motive := fun x ↦
+                      ∀ (h : { toList := head :: x : Array _}.size = 2),
+                        Vector.mk { toList := head :: x } h =
+                        #v[(Vector.mk { toList := head :: x } h)[0], (Vector.mk { toList := head :: x } h)[1]])
+                    (
+                      fun h =>
+                        h.casesOn
+                          (motive := fun a t ↦
+                            2 = a →
+                            h ≍ t →
+                            Vector.mk { toList := [head] } h =
+                            #v[(Vector.mk { toList := [head] } h)[0], (Vector.mk { toList := [head] } h)[1]])
+                          (fun h_1 ↦
+                            Nat.elimOffset (0 + 1) [].length 1 h_1
+                            fun x ↦ False.elim (noConfusion_of_Nat Nat.ctorIdx x))
+                          rfl
+                          HEq.rfl
+                    )
+                    (
+                      fun head_1 tail h ↦
+                        tail.casesOn (motive := fun x ↦
+                          ∀ (h : { toList := head :: head_1 :: x : Array _ }.size = 2),
+                            Vector.mk { toList := head :: head_1 :: x } h =
+                              #v[(Vector.mk { toList := head :: head_1 :: x } h)[0],
+                                (Vector.mk { toList := head :: head_1 :: x } h)[1]])
+                          (fun h ↦ Eq.refl (Vector.mk { toList := [head, head_1] } h))
+                          (fun head_2 tl h ↦
+                            Eq.casesOn (motive := fun a t ↦
+                              2 = a →
+                                h ≍ t →
+                                  Vector.mk { toList := head :: head_1 :: head_2 :: tl } h =
+                                    #v[(Vector.mk { toList := head :: head_1 :: head_2 :: tl } h)[0],
+                                      (Vector.mk { toList := head :: head_1 :: head_2 :: tl } h)[1]])
+                              h
+                              (fun h_1 ↦
+                                Nat.elimOffset (0 + 1) (head_1 :: head_2 :: tl).length 1 h_1 fun x ↦
+                                  Nat.elimOffset 0 (head_2 :: tl).length 1 x fun x ↦
+                                    False.elim (noConfusion_of_Nat Nat.ctorIdx x))
+                              rfl HEq.rfl)
+                  h)
+              )     
+          h
+        )
+        h
 
 /--
 Use with `↓`.
 -/
-dsimproc_decl dontExplodeVector (GetElem.getElem _ _ _) := fun e ↦ do
-  let_expr GetElem.getElem _ _ _ _ _ coll _ _ := e | unreachable!
-  if coll.isFVar
-  then
-    rejectVectorSansProof coll e
-  else 
-    return .continue
-  
+def dontExplodeVector : Sym.Simp.Simproc := fun e ↦ do
+  let_expr GetElem.getElem _ _ _ _ _ coll _ _ := e | return .rfl
+  unless coll.isFVar && (←inferType coll).isAppOf ``Vector do return .rfl
+  trace[Clap.Compile.simp.kaboom] m!"Done:\n{e}"
+  return .rfl (done := true)
+
+/--
+Use with ↑.
+
+TODO: The proof is not `rfl`. One can prove all of these `by aesop (add cases [Vector, Array, List])`,
+      but I'd rather not lift to `aesop` and build the proof by hand (viz. `abc'` above).
+-/
+def explodeVector : Sym.Simp.Simproc := fun e ↦ do
+  let t ← inferType e
+  let_expr Vector t sz := t | return .rfl
+  unless e.isFVar do return .rfl
+  let sz' ← Sym.simp sz
+  match (sz'.getResultExpr sz).nat? with
+  | .none => throwError m!"{sz} does not simplify to ground.\nExpr:\n{e}"
+  | .some n => let explodedVec ← (sequenceAsVecExpr e t n).run'
+               trace[Clap.Compile.simp.kaboom] m!"Exploding:\n{e}\n==>\n{explodedVec}"
+               return .step explodedVec (←mkSorry (←mkEq e explodedVec) false)
+
+def toVectorSequence? (e : Expr) : Sym.Simp.SimpM (Option Expr) := do
+  unless e.isFVar do return .none
+  let_expr Vector t sz := ←inferType e | return .none
+  return .some (←sequenceAsVecExpr e t sz.nat?.get!)
+
+/-
+Ideally, we'd just use `explodeVector` and `dontExplodeVector`
+but marking things `done` in the case of `GetElem ... (.fvar _)` is not quite what the doctor ordered.
+
+Maybe some priority system like in `simp`... for now, we'll just have a `simproc` for each
+of the operations.
+-/
+
+/-
+TODO: Generalise.
+-/
+
+open Compiler.Simp
+
+/--
+TODO: Proof. Viz. `abc'`.
+-/
+def explodeVectorAppend : Sym.Simp.Simproc := fun e ↦ do
+  let_expr HAppend.hAppend _ _ _ _ a b := e | return .rfl
+
+  let a? ← toVectorSequence? a
+  let b? ← toVectorSequence? b
+  if a?.isNone && b?.isNone then return .rfl
+
+  let append ← reducedAndSharedInc (← mkAppM ``HAppend.hAppend #[a?.getD a, b?.getD b])
+  trace[Clap.Compile.simp.kaboom]
+    m!"\n{e}\n==>\n{append}"
+  return .step append (←mkSorry (←mkEq e append) false)
+
+/--
+TODO: Proof. Viz. `abc'`.
+-/
+def explodeVectorMap : Sym.Simp.Simproc := fun e ↦ do
+  let_expr Vector.map _ _ _ f xs := e | return .rfl
+
+  let xs ← toVectorSequence? xs
+  match xs with
+  | .none => return .rfl
+  | .some xs => let map ← reducedAndSharedInc (←mkAppM ``Vector.map #[f, xs])
+                trace[Clap.Compile.simp.kaboom]
+                  m!"\n{e}\n==>\n{map}"
+                return .step map (←mkSorry (←mkEq e map) false)
+
+/--
+TODO: Proof. Viz. `abc'`.
+-/
+def explodeVectorMapM : Sym.Simp.Simproc := fun e ↦ do
+  let_expr Vector.mapM _ _ _ _ _ f xs := e | return .rfl
+  let xs ← toVectorSequence? xs
+  match xs with
+  | .none => return .rfl
+  | .some xs => let map ← reducedAndSharedInc (←mkAppM ``Vector.mapM #[f, xs])
+                trace[Clap.Compile.simp.kaboom]
+                  m!"\n{e}\n==>\n{map}"
+                return .step map (←mkSorry (←mkEq e map) false)
+
+
+-- /--
+-- TODO: Thought experiment to explode on demand.
+
+-- TODO: The proof is not `rfl`. One can prove all of these `by aesop (add cases [Vector, Array, List])`,
+--       but I'd rather not lift to `aesop` and build the proof by hand (viz. `abc'` above).
+
+-- TODO: Can we share state so that we know which lambda was processed?
+-- -/
+-- def explodeVector' : Sym.Simp.Simproc := fun e ↦ do
+--   let Expr.lam name t body _ := e | return .rfl
+--   let_expr Vector t sz := t | return .rfl
+--   let sz' ← Sym.simp sz
+--   match (sz'.getResultExpr sz).nat? with
+--   | .none => throwError m!"{sz} does not simplify to ground"
+--   | .some n =>
+--     -- It's very tricky to get this right using `(.bvar 0)` in `body`. Would it be... faster?
+--     -- Does remaking the lambda break sharing in `Sym`?
+--     lambdaTelescopeOne! e fun arg body ↦ do
+--       logInfo m!"This.\nbinder[{arg}] in: {body}\nt:{t}\nn:{n}\n"
+--       let explodedVec ← (sequenceAsVecExpr arg t n).run' -- Ideally `(.bvar 0)`.
+--       logInfo m!"exploded: {explodedVec}"
+--       trace[Clap.Compile.simp.kaboom] m!"Exploding:\n{e}\n==>\n{explodedVec}"
+--       let body ← Sym.replaceS body fun e _ ↦ do
+--         if !Sym.isSameExpr e arg then return .none -- Does this even trigger?
+--         return .some explodedVec
+--         -- unless e matches .bvar 0 do return .none -- The enclosing binder.
+--       return .step (←Sym.mkLambdaFVarsS #[arg] body) (←Sym.mkEqRefl e) -- Not this proof.
+
 end Clap.Compiler
